{
 "cells": [
  {
   "cell_type": "markdown",
   "metadata": {},
   "source": [
    "# Properties\n",
    "\n",
    "1. [Linearity](https://www.youtube.com/watch?v=0USI-48ovJI&list=PLE8oOccmwGFwDlrfZmJXKZt6tWZKtJvjW&index=3)\n",
    "\n",
    "2. [Conjugate](https://www.youtube.com/watch?v=0USI-48ovJI&list=PLE8oOccmwGFwDlrfZmJXKZt6tWZKtJvjW&index=3)\n",
    "\n",
    "3. [Area under $f(x)$](https://www.youtube.com/watch?v=vshs9v83d0M&list=PLE8oOccmwGFwDlrfZmJXKZt6tWZKtJvjW&index=4)\n",
    "\n",
    "4. [Area under $F(s)$](https://www.youtube.com/watch?v=vshs9v83d0M&list=PLE8oOccmwGFwDlrfZmJXKZt6tWZKtJvjW&index=4)\n",
    "\n",
    "5. [Time reversal (direction reversal)](https://www.youtube.com/watch?v=dWN0DzqlCZk&list=PLE8oOccmwGFwDlrfZmJXKZt6tWZKtJvjW&index=5)\n",
    "6. [Scaling (Similarity)](https://www.youtube.com/watch?v=dWN0DzqlCZk&list=PLE8oOccmwGFwDlrfZmJXKZt6tWZKtJvjW&index=5)\n",
    "\n",
    "7. [Shift](https://www.youtube.com/watch?v=ihfm31HOYJ8&list=PLE8oOccmwGFwDlrfZmJXKZt6tWZKtJvjW&index=6)\n",
    "\n",
    "8. [Frequency shift](https://www.youtube.com/watch?v=ihfm31HOYJ8&list=PLE8oOccmwGFwDlrfZmJXKZt6tWZKtJvjW&index=6)\n",
    "\n",
    "9. [Convolution in time (or space)](https://www.youtube.com/watch?v=khmB0NoJWfA&list=PLE8oOccmwGFwDlrfZmJXKZt6tWZKtJvjW&index=7)\n",
    "\n",
    "10. [Multiplication in time (or space)](https://www.youtube.com/watch?v=t05C3pvLbsc&list=PLE8oOccmwGFwDlrfZmJXKZt6tWZKtJvjW&index=8)\n",
    "\n",
    "11. [Differentiation in time (or space)](https://www.youtube.com/watch?v=mGmPCLUZuGY&list=PLE8oOccmwGFwDlrfZmJXKZt6tWZKtJvjW&index=9)\n",
    "\n",
    "12. [Integration in time (or space)](https://www.youtube.com/watch?v=mGmPCLUZuGY&list=PLE8oOccmwGFwDlrfZmJXKZt6tWZKtJvjW&index=9)\n"
   ]
  },
  {
   "cell_type": "markdown",
   "metadata": {},
   "source": [
    "# Linearity property\n",
    "\n",
    "The Fourier transform of $f_1(x)$ is $F_1(s)$. ie\n",
    "\n",
    "$$ f_1(x) \\leftrightharpoons F_1(s)$$\n",
    "\n",
    "and \n",
    "\n",
    "$$ f_2(x) \\leftrightharpoons F_2(s)$$\n",
    "\n",
    "$a$ and $b$ are constants.  The linearity theorem states that \n",
    "\n",
    "$$a f_1(x) \\leftrightharpoons a F_1(s)$$\n",
    "\n",
    "and\n",
    "\n",
    "$$ b f_2(x) \\leftrightharpoons b F_2(s)$$\n",
    "\n",
    "and \n",
    "\n",
    "$$a f_1(x) + b f_2(x) \\leftrightharpoons a F_1(s) + b F_2(s)$$\n",
    "\n",
    "Proof:\n",
    "\n",
    "let $f(x) = a f_1(x) + b f_2(x)$ and let $f(x) \\leftrightharpoons F(s)$\n",
    "\n",
    "From the formula for Fourier transform we have\n",
    "\n",
    "$$F(s) = \\int \\limits_{-\\infty}^{\\infty} f(x) e^{-2 \\pi i s x} ~dx$$\n",
    "\n",
    "$$F(s) = \\int \\limits_{-\\infty}^{\\infty} [a f_1(x) + b f_2(x)] e^{-2 \\pi i s x} ~dx$$\n",
    "\n",
    "We distribute the exponetial and use the linear property of integrals to write\n",
    "\n",
    "$$F(s) = a \\int \\limits_{-\\infty}^{\\infty} f_1(x) e^{-2 \\pi i s x} ~dx  + b \\int \\limits_{-\\infty}^{\\infty} f_2(x) e^{-2 \\pi i s x} ~dx$$\n",
    "\n",
    "We see that the 1st term on the right is the Fourier transform of $f_1(x)$ and the 2nd term on the right is Fourier transform of $f_2(x)$.  So the Fourier transform is linear because the integration operation is linear. \n",
    "\n",
    "$$F(s) = a F_1(s) + b F_2(s) \\leftrightharpoons f(x) = af_1(x) + b f_2(x)$$\n",
    "\n",
    "QED\n",
    "\n"
   ]
  },
  {
   "cell_type": "markdown",
   "metadata": {},
   "source": [
    "# Conjugation property\n",
    "\n",
    "\n",
    "We begin with a quick review of the conjugate of a product of numbers.\n",
    "\n",
    "Show that the conjugate of a product is the product of the conjugates  \n",
    "\n",
    "$$[(a + ib)(c + id)]^* = (a + ib)^* (c + id)^*$$\n",
    "\n",
    "We expand the left side and take the conguate\n",
    "\n",
    "$$[ac + iad + icb +i^2bd]^* = [(ac - bd) + i(ad +cb)]^* = (ac - bd) - i(ad +cb)$$\n",
    "\n",
    "On the right side we take the conjugate of each factor and then expand\n",
    "\n",
    "$$(a + ib)^* (c + id)^* = (a - ib)(c-id) = ac - iad - ibc + i^2bd =(ac-bd) -i(ad +bc)$$\n",
    "\n",
    "comparing the results from the left and right show that they are the same. \n",
    "QED\n",
    "\n",
    "The conjugation property states that if $f(x) \\leftrightharpoons F(s)$ then  \n",
    "\n",
    "\n",
    "$$f^*(x) \\leftrightharpoons F^*(-s)$$  \n",
    "\n",
    "Proof:\n",
    "\n",
    "$$f(x) \\leftrightharpoons F(s)$$  \n",
    "\n",
    "$$F(s) = \\int \\limits_{-\\infty}^{\\infty} f(x) ~e^{-2 \\pi s x} ~dx $$\n",
    "\n",
    "Recall that the conjugate of a product is the product of the conjugates.  Therefore taking the conjugate of both sides yields.  \n",
    "\n",
    "$$F^*(s) = \\int \\limits_{-\\infty}^{\\infty} f^*(x) ~e^{2 \\pi s x} ~dx $$\n",
    "\n",
    "we now replace $s$ with $-s$ \n",
    "\n",
    "$$s \\rightarrow -s$$\n",
    "\n",
    "$$ F^*(-s) = \\int \\limits_{-\\infty}^{\\infty} f^*(x) ~e^{-2 \\pi s x} ~dx $$\n",
    "\n",
    "\n",
    "\n",
    "$$ F^*(-s) \\leftrightharpoons f^*(x)$$\n",
    "\n",
    "QED\n",
    "\n"
   ]
  },
  {
   "cell_type": "markdown",
   "metadata": {},
   "source": [
    "# Area under $f(x)$\n",
    "\n",
    "The area $A_x$ under the curve $f(x)$ is given by\n",
    "\n",
    "$$A_x = \\int \\limits_{-\\infty}^{\\infty} f(x) ~dx$$\n",
    "\n",
    "The Fourier transform of $f(x)$ is given by\n",
    "\n",
    "$$F(s) = \\int \\limits_{-\\infty}^{\\infty} f(x) e^{-2 \\pi s x} ~dx$$\n",
    "\n",
    "The Fourier transform evaluated at $s=0$ is\n",
    "\n",
    "$$F(0) = \\int \\limits_{-\\infty}^{\\infty} f(x) e^{-2 \\pi (0) x} ~dx = \\int \\limits_{-\\infty}^{\\infty} f(x) ~dx$$\n",
    "\n",
    "$$A_x = F(s) \\big|_{s=0} $$\n",
    "\n",
    "QED\n",
    "\n",
    "From this we see that the \"DC\" value of the signal is simply the area under the curve. \n"
   ]
  },
  {
   "cell_type": "markdown",
   "metadata": {},
   "source": [
    "# Area under $F(s)$\n",
    "\n",
    "The area $A_s$ under the curve in the frequency domain is given by \n",
    "\n",
    "$$ A_s = \\int \\limits_{-\\infty}^{\\infty} F(s) ~ds$$\n",
    "\n",
    "The inverse Fourier transform is given by \n",
    "\n",
    "$$ f(x) = \\frac{1}{2 \\pi} \\int \\limits_{-\\infty}^{\\infty} F(s) e^{2 \\pi s x} ~ds $$\n",
    "\n",
    "Evaluating at $x=0$ yields \n",
    "\n",
    "$$ f(0)= \\frac{1}{2 \\pi} \\int \\limits_{-\\infty}^{\\infty} F(s) e^{2 \\pi s (0)} ~ds = \\frac{1}{2 \\pi} \\int \\limits_{-\\infty}^{\\infty} F(s)  ~ds = \\frac{1}{2 \\pi} A_s$$\n",
    "\n",
    "Therefore \n",
    "\n",
    "$$A_s = 2 \\pi f(x) \\big|_{x=0}$$\n",
    "\n",
    "From this we see that the area under the frequency domain curve is $2 \\pi$ times the signal evaluated at zero.\n",
    "\n",
    "QED"
   ]
  },
  {
   "cell_type": "markdown",
   "metadata": {},
   "source": [
    "# Reversal\n",
    "\n",
    "This property is usually referred to a time reversal, but since we are doing everything in the spatial domain we'll just call it reversal.  Of course, there really is no mathematical difference, we are just using $x$ instead of the $t$.\n",
    "\n",
    "The reversal property states that if\n",
    "\n",
    "$$f(x) \\leftrightharpoons F(s)$$\n",
    "\n",
    "then \n",
    "\n",
    "$$f(-x) \\leftrightharpoons F(-s)$$\n",
    "\n",
    "Proof:\n",
    "\n",
    "$$F(s) = \\int \\limits_{-\\infty}^{\\infty} f(x) ~e^{-2 \\pi s x} ~dx $$\n",
    "\n",
    "We replace $x$ with $-x$\n",
    "\n",
    "$$x \\rightarrow -x$$\n",
    "\n",
    "and let \n",
    "\n",
    "$$F'(s) \\leftrightharpoons f(-x)$$\n",
    "\n",
    "therefore \n",
    "\n",
    "$$F'(s) = \\int \\limits_{-\\infty}^{\\infty} f(-x) ~e^{-2 \\pi s x} ~dx$$\n",
    "\n",
    "Notice that the $x$ in the exponential does <u>not</u> change signs.  We are taking the Fourier transform of a new function (with reversed $x$) but the formula for the Fourier transform does not itself change. \n",
    "\n",
    "Now change the variables:  $-x \\rightarrow \\tau$\n",
    "\n",
    "$$-x = \\tau \\Rightarrow x = -\\tau \\Rightarrow dx = -d\\tau$$\n",
    "\n",
    "We change the limits of integration\n",
    "\n",
    "$$x = -\\infty \\Rightarrow \\tau = \\infty $$\n",
    "$$x = \\infty \\Rightarrow \\tau = -\\infty$$\n",
    "\n",
    "Putting this together simplying, we have the following.  *Notice that the minus sign in front of $d\\tau$ comes outside the integral and is then canceled by reversing the order of integration.*\n",
    "\n",
    "$$F'(s) = \\int \\limits_{\\infty}^{-\\infty} f(\\tau) ~e^{-2 \\pi s (-\\tau)} ~(-d\\tau)= -\\int \\limits_{\\infty}^{-\\infty} f(\\tau) ~e^{2 \\pi s \\tau} ~d\\tau = \\int \\limits_{-\\infty}^{\\infty} f(\\tau) ~e^{2 \\pi s \\tau} ~d\\tau $$\n",
    "\n",
    "In order to have the Fourier transform we introduce a minus sign in the exponential but change the sign of $s$ to maintain equality. \n",
    "\n",
    "$$F'(s) = \\int \\limits_{-\\infty}^{\\infty} f(\\tau)~ e^{-2 \\pi (-s) \\tau} ~d\\tau $$\n",
    "\n",
    "Therefore, from observation we have \n",
    "\n",
    "$$F'(s) = F(-s)$$\n",
    "\n",
    "and\n",
    "\n",
    "$$f(-x) \\leftrightharpoons F(-s)$$\n",
    "\n",
    "QED\n"
   ]
  },
  {
   "cell_type": "markdown",
   "metadata": {},
   "source": [
    "# Similarity\n",
    "\n",
    "The similarity theorem states that if\n",
    "\n",
    "$$f(x) \\leftrightharpoons F(s)$$\n",
    "\n",
    "then \n",
    "\n",
    "$$f(ax) \\leftrightharpoons \\frac{1}{|a|} F\\Big(\\frac{s}{a}\\Big)$$\n",
    "\n",
    "where $a$ is any real number except for zero.\n",
    "\n",
    "Proof:\n",
    "\n",
    "The formula for the Fourier transfrom is\n",
    "\n",
    "$$F(s) = \\int \\limits_{-\\infty}^{\\infty} f(x) e^ {-2 \\pi i s x} ~dx$$\n",
    "\n",
    "We scale $f(x)$ by $a$\n",
    "\n",
    "$$f(x) \\rightarrow f(ax)$$\n",
    "\n",
    "Where $a$ is a real, non zero number. \n",
    "\n",
    "We would like to find\n",
    "\n",
    "$$F'(s) \\leftrightharpoons f(ax)$$\n",
    "\n",
    "There are two cases: $a>0$ and $a<0$\n",
    "\n",
    "Case I: $a>0$\n",
    "\n",
    "$$F'(s) = \\int \\limits_{-\\infty}^{\\infty} f(ax) ~e^{-2 \\pi s x} ~dx $$\n",
    "\n",
    "let $u = ax \\Rightarrow x = \\frac{u}{a} \\Rightarrow dx = \\frac{du}{a}$\n",
    "\n",
    "The limits of integration do not change when we make the substitution\n",
    "\n",
    "$$F'(s) = \\int \\limits_{-\\infty}^{\\infty} f(u) ~e^{-2 \\pi s (\\frac{u}{a})} ~\\frac{du}{a}$$\n",
    "\n",
    "Now we associate $a$ with $s$ and bring the constant $\\frac{1}{a}$ outside the integral to get\n",
    "\n",
    "\n",
    "\n",
    "$$F'(s) = \\frac{1}{a} \\int \\limits_{-\\infty}^{\\infty} f(u) ~e^{-2 \\pi (\\frac{s}{a})u } ~du$$\n",
    "\n",
    "Therefore, by observation, \n",
    "\n",
    "$$F'(s) = \\frac{1}{a} F\\Big(\\frac{s}{a}\\Big)$$\n",
    "\n",
    "Case II: $a<0$\n",
    "\n",
    "To account for the case where $a<0$ we take the absolute value of $a$\n",
    "\n",
    "$$F'(s) = \\frac{1}{|a|} F\\Big(\\frac{s}{a}\\Big)$$\n",
    "\n",
    "Therefore \n",
    "\n",
    "$$f(ax) \\leftrightharpoons \\frac{1}{|a|} F \\Big(\\frac{s}{a} \\Big) $$\n",
    "\n",
    "QED"
   ]
  },
  {
   "cell_type": "markdown",
   "metadata": {},
   "source": [
    "# Shift"
   ]
  },
  {
   "cell_type": "markdown",
   "metadata": {},
   "source": [
    "The shift theorem states that if \n",
    "\n",
    "$$f(x) \\leftrightharpoons F(s)$$\n",
    "\n",
    "then \n",
    "\n",
    "$$f(x \\pm x_o) \\leftrightharpoons e^{\\pm 2 \\pi i x_o} F(s)$$"
   ]
  },
  {
   "cell_type": "markdown",
   "metadata": {},
   "source": [
    "Proof:\n",
    "\n",
    "The Fourier transform of $f(x)$ is given by\n",
    "\n",
    "$$F(s) = \\int \\limits_{-\\infty}^{\\infty} f(x) e^{-2 \\pi i x s} ~dx $$\n",
    "\n",
    "We shift the function to the right by replacing $x$ with $(x-x_o)$.  \n",
    "\n",
    "$$x \\rightarrow (x-x_o)$$\n",
    "\n",
    "$$f(x) \\rightarrow f(x-x_o)$$ \n",
    "\n",
    "We call the Fourier transform of the shifted function $F'(s)$\n",
    "\n",
    "$$F'(s) = \\int \\limits_{-\\infty}^{\\infty} f(x-x_o) ~e^{-2 \\pi i s x} ~dx$$\n",
    "\n",
    "let $u=x-x_o \\Rightarrow x = u + x_o \\Rightarrow dx = du$"
   ]
  },
  {
   "cell_type": "markdown",
   "metadata": {},
   "source": [
    "$$F'(s) = \\int \\limits_{-\\infty}^{\\infty} f(u) ~e^{-2 \\pi i s (u + x_o)} ~du$$\n",
    "\n",
    "We separate the exponential\n",
    "\n",
    "$$F'(s) = \\int \\limits_{-\\infty}^{\\infty} f(u) ~e^{-2 \\pi i s u}~e^{-2 \\pi i s x_o} ~du$$\n",
    "\n",
    "The exponential with $x_o$ is a constant with respect to $u$ so it comes out of the integral. We recognize that what remains in the integral is the Fourier transform of the signal. \n",
    "\n",
    "$$F'(s) = e^{-2 \\pi s i x_o}\\int \\limits_{-\\infty}^{\\infty} f(u) ~e^{-2 \\pi i s u} ~du = e^{-2 \\pi i s x_o} F(s)$$\n",
    "\n",
    "Therefore \n",
    "\n",
    "$$f(x\\pm x_o) \\leftrightharpoons e^{\\pm2 \\pi i s x_o} F(s)$$\n",
    "\n",
    "QED\n",
    "\n",
    "Notice that when the shift is to the right, ie $(x-x_o)$, the exponential has a negative sign and when the shift is to the left, ie $(x+x_o)$, the exponential has a positive sign.\n"
   ]
  },
  {
   "cell_type": "markdown",
   "metadata": {},
   "source": [
    "# Frequency shift\n",
    "\n",
    "The frequency shift states that if $f(x) \\leftrightharpoons F(s)$ then \n",
    "\n",
    "$$e^{\\pm 2 \\pi i s_o x} f(x) \\leftrightharpoons F(s \\mp s_o) $$\n",
    "\n",
    "Proof:  \n",
    "The Fourier transform of $f(x)$ is\n",
    "\n",
    "$$F(s) = \\int \\limits_{-\\infty}^{\\infty} f(x) ~e^{-2 \\pi i s x} ~dx $$\n",
    "\n",
    "We refer to the Fourier transform of the phase shifted function $F'(s)$\n",
    "\n",
    "$$e^{2 \\pi i s_o x} f(x) \\leftrightharpoons F'(s) $$\n",
    "\n",
    "We apply the Fourier transform formula to the phase shifted signal"
   ]
  },
  {
   "cell_type": "markdown",
   "metadata": {},
   "source": [
    "$$F'(s) = \\int \\limits_{-\\infty}^{\\infty} e^{2 \\pi i s_o x} f(x) ~e^{-2 \\pi i s x} ~dx$$\n",
    "\n",
    "and combine the exponentials"
   ]
  },
  {
   "cell_type": "markdown",
   "metadata": {},
   "source": [
    "$$F'(s) = \\int \\limits_{-\\infty}^{\\infty} f(x) ~e^{-2 \\pi i (s-s_o) x}  ~dx$$\n",
    "\n",
    "By observation\n",
    "\n",
    "$$F'(s) = F(s-s_o) \\leftrightharpoons e^{2 \\pi i s_o x} f(x) $$\n",
    "\n",
    "\n",
    "Notice that if the frequency is shifted to the left the equation has the opposite sign.  Therefore\n",
    "\n",
    "$$F'(s) = F(s\\mp s_o) \\leftrightharpoons e^{\\pm 2 \\pi i s_o x} f(x) $$\n",
    "\n",
    "QED\n"
   ]
  },
  {
   "cell_type": "markdown",
   "metadata": {},
   "source": [
    "# Convolution in space (or time)\n",
    "\n",
    "Before we show the convolution theorem we will state the definition of convolution. We will use $*$ to indicate convolution. $f(x)$ convolved with $g(x)$ is written as \n",
    "\n",
    "$$ f(x) ~*~ g(x) = \\int \\limits_{-\\infty}^{\\infty} f(\\tau) g(x-\\tau) ~d\\tau$$\n",
    "\n",
    "$\\tau$ is dummy variable that's used to keep things straight in the integral\n"
   ]
  },
  {
   "cell_type": "markdown",
   "metadata": {},
   "source": [
    "Given two functions, each with it's corresponding Fourier transforms:\n",
    "\n",
    "$$f(x) \\leftrightharpoons F(s)$$\n",
    "$$g(x) \\leftrightharpoons G(s)$$\n",
    "\n",
    "The convolution theorem states that\n",
    "\n",
    "$$f(x) ~*~ g(x) \\leftrightharpoons F(s) ~G(s)$$\n",
    "\n",
    "That is, convolution in the spatial domain is equivalent to multiplication in the spatial frequency domain. \n",
    "\n"
   ]
  },
  {
   "cell_type": "markdown",
   "metadata": {},
   "source": [
    "Proof: \n",
    "\n",
    "let $h(x) = f(x) ~*~ g(x)$\n",
    "\n",
    "$$h(x) \\leftrightharpoons H(s)$$\n",
    "\n",
    "The Fourier transform of $h(x)$ is given by\n",
    "\n",
    "$$H(s) = \\int \\limits_{-\\infty}^{\\infty} h(x) ~e^{-2 \\pi s x} ~dx $$\n",
    "\n",
    "Substituting the equation for $h(x)$ into the formula yields\n",
    "\n",
    "$$H(s) = \\int \\limits_{-\\infty}^{\\infty} \\Bigg[ \\int \\limits_{-\\infty}^{\\infty} f(\\tau) g(x-\\tau) ~d\\tau \\Bigg] e^{- 2 \\pi i s x} ~dx$$\n",
    "\n"
   ]
  },
  {
   "cell_type": "markdown",
   "metadata": {},
   "source": [
    "let $x-\\tau = \\lambda \\Rightarrow x = \\lambda + \\tau \\Rightarrow dt = d\\lambda$. \n",
    "\n",
    "The range of integration is same after substitution\n",
    "\n",
    "$$H(s) = \\int \\limits_{-\\infty}^{\\infty}  \\int \\limits_{-\\infty}^{\\infty} f(\\tau) g(\\lambda) ~d\\tau  ~e^{- 2 \\pi i s (\\lambda + \\tau)} ~d\\lambda$$\n",
    "\n",
    "We separate the exponential\n",
    "\n",
    "$$H(s) = \\int \\limits_{-\\infty}^{\\infty}  \\int \\limits_{-\\infty}^{\\infty} f(\\tau) g(\\lambda) ~d\\tau  ~e^{- 2 \\pi i s \\lambda}  ~e^{- 2 \\pi i s\\tau} ~d\\lambda$$\n",
    "\n",
    "We rearrange by grouping factors with $\\tau$ together and grouping factors with $\\lambda$ together to yield\n"
   ]
  },
  {
   "cell_type": "markdown",
   "metadata": {},
   "source": [
    "$$H(s) = \\int \\limits_{-\\infty}^{\\infty} f(\\tau) ~e^{- 2 \\pi i s\\tau} ~d\\tau\\int \\limits_{-\\infty}^{\\infty}  g(\\lambda)   e^{- 2 \\pi i s \\lambda} ~d\\lambda$$\n",
    "\n",
    "From this we see that the integral associated with $\\tau$ is the Fourier transform of $f(x)$ and the integral associated with $\\lambda$ is the Fourier transform of $g(x)$. "
   ]
  },
  {
   "cell_type": "markdown",
   "metadata": {},
   "source": [
    "$$ H(s) = F(s) G(s) \\leftrightharpoons f(x) ~*~ g(x) $$\n",
    "\n",
    "QED\n",
    "\n",
    "This property is useful in computing convolutions.  We can multiply the Fourier transforms of two functions and take the inverse Fourier transform to find the convolution $h(x)$"
   ]
  },
  {
   "cell_type": "markdown",
   "metadata": {},
   "source": [
    "# Mulitplication in space\n",
    "\n",
    "Also known as convolution in spatial frequency. "
   ]
  },
  {
   "cell_type": "markdown",
   "metadata": {},
   "source": [
    "For two functions with their cooresponding Fourier transforms\n",
    "\n",
    "$$f(x) \\leftrightharpoons F(s)$$\n",
    "$$g(x) \\leftrightharpoons G(s)$$\n",
    "\n",
    "The convolution in spatial frequency theorem states that \n",
    "\n",
    "$$ f(x) g(x) \\leftrightharpoons \\frac{1}{2 \\pi} \\Big| F(s) ~*~ G(s) \\Big| $$"
   ]
  },
  {
   "cell_type": "markdown",
   "metadata": {},
   "source": [
    "To prove the theorm above we consider the Fourier transform (FT) of the product of functions in the spatial domain\n",
    "\n",
    "$$\\text{FT} \\Big[ f(x) g(x) \\Big] = \\frac{1}{2 \\pi} \\Big[ F(s) ~*~ G(s) \\Big] $$ \n",
    "\n",
    "Taking the inverse Fourier transform (IFT) of both sides gives us\n",
    "\n",
    "$$ f(x) g(x) = \\text{IFT} \\Big[ \\frac{1}{2 \\pi} \\Big( F(s) ~*~ G(s) \\Big) \\Big] $$\n",
    "\n",
    "Therefore proving that this is true is the same as proving the theorem. "
   ]
  },
  {
   "cell_type": "markdown",
   "metadata": {},
   "source": [
    "Let $H(s) = \\frac{1}{2 \\pi} \\big(F(s) ~*~ G(s)\\big) \\leftrightharpoons h(x) = f(x)g(x)$\n",
    "\n",
    "so\n",
    "\n",
    "$$h(x) = \\text{IFT} \\Big[H(s) \\Big] = \\frac{1}{2 \\pi} \\int \\limits_{-\\infty}^{\\infty} H(s) e^{2 \\pi i s x} ~ds $$"
   ]
  },
  {
   "cell_type": "markdown",
   "metadata": {},
   "source": [
    "We express the convolution directly from the defintion\n",
    "\n",
    "$$H(s) = \\frac{1}{2 \\pi} \\int \\limits_{-\\infty}^{\\infty} F(\\lambda) G(s-\\lambda)~d\\lambda$$\n",
    "\n",
    "We substitute this into the equation for $h(x)$\n",
    "\n"
   ]
  },
  {
   "cell_type": "markdown",
   "metadata": {},
   "source": [
    "$$h(x)  = \\frac{1}{2 \\pi} \\int \\limits_{-\\infty}^{\\infty} \\Bigg[\\frac{1}{2 \\pi} \\int \\limits_{-\\infty}^{\\infty} F(\\lambda) G(s-\\lambda)~d\\lambda \\Bigg] e^{2 \\pi i s x} ~ds $$\n",
    "\n",
    "Rearranging yields\n",
    "$$h(x)  = \\Bigg(\\frac{1}{2 \\pi}\\Bigg)^2 \\int \\limits_{-\\infty}^{\\infty} \\int \\limits_{-\\infty}^{\\infty} F(\\lambda) G(s-\\lambda)~d\\lambda  ~e^{2 \\pi i s x} ~ds $$\n",
    "\n",
    "\n",
    "\n",
    "Next we multiply by $\\frac{e^{2 \\pi i\\lambda x}}{e^{2 \\pi i\\lambda x}}$\n",
    "\n",
    "$$h(x)  = \\Bigg(\\frac{1}{2 \\pi}\\Bigg)^2 \\int \\limits_{-\\infty}^{\\infty} \\int \\limits_{-\\infty}^{\\infty} F(\\lambda) G(s-\\lambda)~d\\lambda  ~e^{2 \\pi i s x} ~ds ~\\frac{e^{2 \\pi i\\lambda x}}{e^{2 \\pi i\\lambda x}}$$\n",
    "\n",
    "We associate the exponential in the numerator with $F(\\lambda)$ and the exponetial in the denominator with $G(s-\\lambda)$. "
   ]
  },
  {
   "cell_type": "markdown",
   "metadata": {},
   "source": [
    "$$h(x)  = \\Bigg(\\frac{1}{2 \\pi}\\Bigg)^2 \\int \\limits_{-\\infty}^{\\infty} F(\\lambda) ~e^{2 \\pi i\\lambda x}~d\\lambda \\int \\limits_{-\\infty}^{\\infty}  G(s-\\lambda)  ~e^{2 \\pi i s x} ~e^{-2 \\pi i\\lambda x} ~ds$$\n",
    "\n",
    "We combine the two exponetials associated with $G(s-\\lambda)$\n",
    "\n",
    "$$h(x)  = \\Bigg(\\frac{1}{2 \\pi}\\Bigg)^2 \\int \\limits_{-\\infty}^{\\infty} F(\\lambda) ~e^{2 \\pi i\\lambda x}~d\\lambda \\int \\limits_{-\\infty}^{\\infty}  G(s-\\lambda)  ~e^{2 \\pi i (s-\\lambda) x}  ~ds$$"
   ]
  },
  {
   "cell_type": "markdown",
   "metadata": {},
   "source": [
    "now we let $u = s - \\lambda \\Rightarrow du = ds$.  Substituing these into the equation and associating a $\\frac{1}{2 \\pi}$ with each integral gives us \n",
    "\n"
   ]
  },
  {
   "cell_type": "markdown",
   "metadata": {},
   "source": [
    "$$h(x)  = \\frac{1}{2 \\pi} \\int \\limits_{-\\infty}^{\\infty} F(\\lambda) ~e^{2 \\pi i\\lambda x}~d\\lambda ~\\frac{1}{2 \\pi} \\int \\limits_{-\\infty}^{\\infty}  G(u)  ~e^{2 \\pi i u x}  ~du$$\n",
    "\n",
    "In this form we can see that the 1st integral is the IFT of $F(s)$ and the 2nd is the IFT of $G(s)$\n",
    "\n",
    "Therefore we have shown that a convolution in spatial frequency is equivilent to a multiplication in space\n",
    "\n",
    "$$h(x) = f(x) ~g(x) \\leftrightharpoons \\frac{1}{2 \\pi} \\Bigg| F(s) ~*~ G(s) \\Bigg|$$\n",
    "\n",
    "QED"
   ]
  },
  {
   "cell_type": "markdown",
   "metadata": {},
   "source": [
    "# Differentiation in space\n",
    "\n",
    "For a function $f(x)$ with a Fourier transform $F(s)$\n",
    "\n",
    "$$ f(x) \\leftrightharpoons F(s)$$\n",
    "\n",
    "$$ \\frac{~d}{dx} f(x) \\leftrightharpoons 2 \\pi i s F(s)$$\n",
    "\n",
    "And in general \n",
    "\n",
    "$$\\frac{d^k}{dx^k} f(x) \\leftrightharpoons (2 \\pi i s)^k F(s)$$\n",
    "\n",
    "Proof:\n",
    "\n",
    "The signal function $f(x)$ is expressed as an inverse Fourier transform:\n",
    "\n",
    "$$ f(x) = \\frac{1}{2 \\pi } \\int \\limits_{-\\infty}^{\\infty} F(s) ~e^{2 \\pi i s x} ~ds$$\n",
    "\n",
    "Taking the derivative with respect to $x$ of both sides yeilds\n",
    "\n",
    "$$ \\frac{~d}{dx} f(x) =  \\frac{~d}{dx} \\Bigg[\\frac{1}{2 \\pi } \\int \\limits_{-\\infty}^{\\infty} F(s) ~e^{2 \\pi i s x} ~ds \\Bigg]$$\n",
    "\n",
    "\n",
    "Because only the exponetial is a function of $x$ all else is treated as a constant.  Applying the chain rule when taking the derivative gives us \n",
    "\n",
    "$$ \\frac{~d}{dx} f(x) =  \\frac{1}{2 \\pi } \\int \\limits_{-\\infty}^{\\infty} F(s) (2 \\pi i s) ~e^{2 \\pi i s x} ~ds$$\n",
    "\n",
    "Bringing the constant outside the integrals let's us see that the derivative of the inverse Fourier transform is simply the inverse Fourier transform multiplied by $2 \\pi i s$\n",
    "\n",
    "$$ \\frac{~d}{dx} f(x) = (2 \\pi i s) \\frac{1}{2 \\pi } \\int \\limits_{-\\infty}^{\\infty} F(s)  ~e^{2 \\pi i s x} ~ds $$\n",
    "\n",
    "Therefore\n",
    "\n",
    "$$\\frac{~d}{dx} f(x) \\leftrightharpoons 2 \\pi i s F(s) $$\n",
    "\n",
    "QED"
   ]
  },
  {
   "cell_type": "markdown",
   "metadata": {},
   "source": []
  },
  {
   "cell_type": "code",
   "execution_count": null,
   "metadata": {},
   "outputs": [],
   "source": []
  }
 ],
 "metadata": {
  "kernelspec": {
   "display_name": "Python 3",
   "language": "python",
   "name": "python3"
  },
  "language_info": {
   "codemirror_mode": {
    "name": "ipython",
    "version": 3
   },
   "file_extension": ".py",
   "mimetype": "text/x-python",
   "name": "python",
   "nbconvert_exporter": "python",
   "pygments_lexer": "ipython3",
   "version": "3.7.6"
  }
 },
 "nbformat": 4,
 "nbformat_minor": 4
}
